added bound restriction on segfree; will remove now, come back to here if needed

theories/operations.v
@@ -209,11 +209,11 @@ End l_is_s.
 
 
 
-Inductive sfree : segment -> allocator -> N -> N -> segment -> allocator -> Prop :=
-  Free : forall T A a nid l n A',
+Inductive sfree : segment -> allocator -> N -> N -> N -> segment -> allocator -> Prop :=
+  Free : forall T A a n nid l A',
       find_and_remove nid A.(allocated) = Some (l, a, n) ->
       A' = {| allocated := l; next_free := next_free A |} ->
-      sfree T A a nid T A'.
+      sfree T A a n nid T A'.
 
 
   
