theories/interpreter_func.v
@@ -552,27 +552,15 @@ with run_one_step (fuel : fuel) (d : depth) (cfg : config_one_tuple_without_e) (
 
   | AI_basic BI_segfree =>
       if ves is VAL_handle h :: ves' then
-(*        expect
-          (sseg_ind s f.(f_inst))
-          (fun j =>
-             expect
-               (sall_ind s f.(f_inst))
-               (fun j' =>
-                  if List.nth_error s.(s_segs) j is Some s_seg_s_j then
-                    if List.nth_error s.(s_alls) j' is Some s_all_s_j' then *)
-                      if h.(valid) && (N.eqb h.(offset) N.zero) then
-                        expect
-                          (find_and_remove h.(id) s.(s_alls).(allocated))
-                          (fun '(l, a, n) =>
-                             if (N.eqb a h.(base)) then
-                               (upd_s_all s {| allocated := l; next_free := next_free s.(s_alls) |}, f, RS_normal (vs_to_es ves'))
-                             else (s, f, crash_error))
-                          ((s, f, crash_error))
-                      else (s, f, crash_error)
-(*                    else (s, f, crash_error)
-                  else (s, f, crash_error))
-               ((s, f, crash_error)))
-          ((s, f, crash_error)) *)
+        if h.(valid) && (N.eqb h.(offset) N.zero) then
+          expect
+            (find_and_remove h.(id) s.(s_alls).(allocated))
+            (fun '(l, a, n) =>
+               if (N.eqb a h.(base) && N.eqb n h.(bound)) then
+                 (upd_s_all s {| allocated := l; next_free := next_free s.(s_alls) |}, f, RS_normal (vs_to_es ves'))
+               else (s, f, crash_error))
+            ((s, f, crash_error))
+        else (s, f, crash_error)
       else (s, f, crash_error)
 
 
